theories/rust_typing/shr_ref/deinit.v
@@ -29,7 +29,7 @@ Section deinit.
     iExists tt. iR.
     iModIntro. iExists l'. iFrame. rewrite uninit_own_spec. iExists ly.
     apply syn_type_has_layout_ptr_inv in Halg as ->. iSplitR; last done.
-    iPureIntro. destruct Hstcomp as [<- | (ly1 & Hst' & ->)]; first done.
+    iPureIntro. destruct Hstcomp as [<- | (ly1 & Hst' & ->)]; first by apply syn_type_has_layout_ptr.
     specialize (syn_type_has_layout_ptr_inv _ Hst') as ->.
     eapply syn_type_has_layout_make_untyped; done.
   Qed.
@@ -57,7 +57,7 @@ Section deinit.
     iExists tt. iR.
     iModIntro. iExists l'. iFrame. rewrite uninit_own_spec. iExists ly.
     apply syn_type_has_layout_ptr_inv in Halg as ->. iSplitR; last done.
-    iPureIntro. destruct Hstcomp as [<- | (ly1 & Hst' & ->)]; first done.
+    iPureIntro. destruct Hstcomp as [<- | (ly1 & Hst' & ->)]; first by apply syn_type_has_layout_ptr.
     specialize (syn_type_has_layout_ptr_inv _ Hst') as ->.
     eapply syn_type_has_layout_make_untyped; done.
   Qed.
